Weidenbach_Book/Watched_Literals_Watch_List_Domain_Restart.thy
@@ -2,6 +2,7 @@ theory Watched_Literals_Watch_List_Domain_Restart
   imports Watched_Literals_Watch_List Watched_Literals_Watch_List_Restart
 begin
 
+
 lemma cdcl_twl_restart_get_all_init_clss:
   assumes \<open>cdcl_twl_restart S T\<close>
   shows \<open>get_all_init_clss T = get_all_init_clss S\<close>
